proof/jasmin_extracts/Uniform_distr_extract_ct.ec
@@ -1,0 +1,12 @@
+require import AllCore IntDiv CoreMap List Distr.
+require import JModel.
+
+
+
+
+module M = {
+  var leakages : leakages_t
+  
+  
+}.
+
